src/unitb/models/simple.lean
@@ -18,25 +18,34 @@ structure program : Type :=
   (first : α)
   (step : α → α)
 
-def pred := α → Prop
+def pred := pred' α
 
 parameter {α}
 
 def program.init (s : program) (p : pred) : Prop :=
-p (s^.first)
+s.first ⊨ p
+
+def is_step (s : program) (σ σ' : α) : Prop := σ' = s.step σ
 
 def program.transient (s : program) (p q : pred) : Prop :=
-∀ σ, p σ → q σ → ¬ (q (s^.step σ))
+⊩ ⟦is_step s⟧ ⟶ •p ⟶ •q ⟶ ⊙-•q
 
 def program.unless (s : program) (p q : pred) : Prop :=
-∀ σ, p σ ∧ ¬q σ → p (s^.step σ) ∨ q (s^.step σ)
+∀ σ, σ ⊨ p ∧ ¬σ ⊨ p → s.step σ ⊨ p ∨ s.step σ ⊨ q
+
+open temporal
 
 lemma program.transient_impl (s : program) {p q : pred}
   (H : p ⟹ -q)
 : s.transient p q :=
-begin
-  intros σ hp hq,
-  cases H _ hp hq,
+begin [temporal]
+  intros STEP hp hq,
+  exfalso,
+  revert hq hp,
+  simp, rw [not_init],
+  clear STEP,
+  show _,
+  { revert Γ, change _ ⟹ _, monotonicity H, },
 end
 
 lemma program.transient_antimono (s : program) (p q p' q' : pred)
@@ -44,14 +53,16 @@ lemma program.transient_antimono (s : program) (p q p' q' : pred)
   (hq : q' ⟹ q)
   (T₀ : s.transient p q)
 : s.transient p' q' :=
-begin
-  intros σ hp' hq',
-  have h'' := T₀ σ (hp _ hp') (hq _ hq'),
-  intro h₂, apply h'',
-  apply hq _ h₂
+begin [temporal]
+  replace hp := init_entails_init hp,
+  replace hq := init_entails_init hq,
+  intros STEP hp' hq',
+  replace T₀ := T₀ Γ STEP (hp Γ hp') (hq Γ hq'),
+  revert T₀,
+  persistent,
+  monotonicity,
+  apply hq,
 end
-
-def is_step (s : program) (σ σ' : α) : Prop := σ' = s.step σ
 
 instance prog_is_system : system program :=
   { σ := α
@@ -65,8 +76,8 @@ instance prog_is_system : system program :=
 lemma unless_step
   {init : α}
   {step : α → α}
-  {p q : α → Prop}
-  (h : ∀ σ, p σ → ¬ q σ → p (step σ) ∨ q (step σ))
+  {p q : pred}
+  (h : ∀ σ, σ ⊨ p → ¬ σ ⊨ q → step σ ⊨ p ∨ step σ ⊨ q)
 : unless (program.mk init step) p q :=
 begin
   unfold unless,
@@ -85,15 +96,17 @@ lemma leads_to_step
   (init : α)
   (step : α → α)
   (p q : pred)
-  (h : ∀ σ, p σ → ¬ q σ → q (step σ))
+  (h : ∀ σ, σ ⊨ p → ¬ σ ⊨ q → step σ ⊨ q)
 : p ↦ q in program.mk init step :=
 begin
   apply leads_to.basis,
-  { intros σ _ h,
-    cases h with h₀ h₁,
-    have h' := h _ h₀ h₁,
-    simp [not_and_iff_not_or_not,not_not_iff_self],
-    left, apply h', },
+  { lifted_pred,
+    intros,
+    simp [p_not_p_and,p_not_p_not_iff_self],
+    cases p, cases q,
+    simp [next,temporal.init,stream.tail,action,is_step] at *,
+    specialize h _ a_1 a_2,
+    left, simp [a,h], },
   { apply unless_step,
     intros σ hp hnq,
     right, apply h _ hp hnq, }
@@ -106,69 +119,66 @@ open temporal
 def ex (s : program) : cpred α :=
 •eq s.first ⋀ ◻ ⟦ is_step s ⟧
 
-lemma ex.safety {s : program} (τ : stream α)
-  (h : ex s τ)
-: ◻ ⟦ is_step s ⟧ $ τ :=
-h.right
+lemma ex.safety (s : program)
+: ex s ⟹ ◻ ⟦ is_step s ⟧ :=
+begin [temporal]
+  intros h, apply h.right
+end
 
 def ex.witness (s : program) : stream α
   | 0 := s.first
   | (succ i) := s.step (ex.witness i)
 
 lemma ex.witness_correct (s : program)
-: ex s (ex.witness s) :=
+: ex.witness s ⊨ ex s :=
 begin
   unfold ex, simp,
   split,
   { intro i,
-    rw action_drop,
-    unfold is_step,
+    simp [action,is_step,stream.drop],
     refl },
-  { unfold temporal.init,
-    refl }
+  { simp [temporal.init],
+    exact rfl }
 end
 
 section semantics
 
 variable {s : program}
+variable Γ : cpred α
 variables {p q : pred}
-variable τ : stream α
-variable (H : ex s τ)
+variables H : Γ ⊢ ex s
 open temporal
-
 include H
 
 lemma init_sem
   (I₀ : init s p)
-: (•p) τ :=
-begin
-  unfold temporal.init,
+: Γ ⊢ •p :=
+begin [temporal]
   have H' := H.left,
-  unfold temporal.init at H',
-  rw ← H', apply I₀,
+  revert H',
+  lifted_pred,
+  show _ ,
+  { intros,
+    unfold_coes at a_1,
+    simp [temporal.init] at a_1 ⊢,
+    rw ← a_1,
+    assumption },
 end
 
 lemma transient.semantics
   (T₀ : transient' s p q)
-: (◻◇•p) τ → (◻◇•-q) τ :=
-begin
+: Γ ⊢ ◻◇•p ⟶ ◻◇-•q :=
+begin [temporal]
   intros Hp,
-  have Hstep : (◇◻⟦is_step s⟧) τ,
-  { apply eventually_weaken,
-    apply ex.safety τ H },
-  have H' := coincidence Hstep Hp,
+  replace H := coincidence' (ex.safety s Γ H) Hp,
   rw ← eventually_eventually,
-  apply inf_often_entails_inf_often _ _ H',
-  { unfold p_entails, rw p_and_p_imp,
-    intros τ Hs Hp,
-    cases classical.em (•q $ τ) with Hq Hnq,
-    { apply eventually_of_next,
-      dsimp [transient',system.transient,simple.program.transient] at T₀,
-      unfold action is_step at Hs,
-      rw [next_init,Hs],
-      apply T₀ _ Hp Hq, },
-    { rw [← p_not_to_fun,not_init] at Hnq,
-      apply eventually_weaken _ Hnq }, },
+  revert H,
+  monotonicity,
+  { rw p_and_p_imp,
+    intros Hs Hp,
+    cases predicate.em (•q) with Hq Hnq,
+    { apply T₀ Γ Hs Hp Hnq, },
+    { apply Hq } },
 end
 
 end semantics
