src/unitb/refinement/basic.lean
@@ -24,8 +24,8 @@ infix ` ⊑ `:80 := refined
 def data_ref [system_sem α] [system_sem β]
     (s : α)  (f : unitb.state α  → σ)
     (s' : β) (g : unitb.state β  → σ) : Prop :=
-∀ τ : stream (unitb.state β), system_sem.ex s' τ
-→ ∃ τ', system_sem.ex s τ' ∧ (g ∘ τ) = (f ∘ τ')
-
+∀ τ : stream (unitb.state β),
+        τ  ⊨ system_sem.ex s'
+→ ∃ τ', τ' ⊨ system_sem.ex s ∧ (g ∘ τ) = (f ∘ τ')
 
 end unitb.refinement
